Splinter/MsgHistory.i.dfy
@@ -73,6 +73,7 @@ module MsgHistoryMod {
       requires other.WF()
       requires IsEmpty() || other.IsEmpty() || other.seqStart == seqEnd
       ensures result.WF()
+      ensures result.LSNSet() == LSNSet() + other.LSNSet()
       // conditions on msgSeq bounds
     {
       if IsEmpty()
